Full Core of Higher Order Contracts. No automation for now

state/HigherOrderContracts.fst
@@ -97,6 +97,14 @@ instance exportable_sum t1 t2 {| c1:exportable_from t1 |} {| c2:exportable_from 
     match x with | Inl x -> c1.lemma_export_preserves_prref x | Inr x -> c2.lemma_export_preserves_prref x)
 }
 
+instance exportable_resexn t {| c:exportable_from t |} : exportable_from (resexn t) = {
+  c_styp = witnessable_sum t err #c.c_styp;
+  ityp = resexn c.ityp;
+  c_ityp = targetlang_sum default_spec c.ityp err #c.c_ityp;
+  export = (fun x -> match x with | Inl x -> Inl (c.export x) | Inr err -> Inr err);
+  lemma_export_preserves_prref = (fun x -> match x with | Inl x -> c.lemma_export_preserves_prref x | Inr err -> ())
+}
+
 instance exportable_pair t1 t2 {| c1:exportable_from t1 |} {| c2:exportable_from t2 |} : exportable_from (t1 * t2) = {
   c_styp = witnessable_pair t1 t2 #c1.c_styp #c2.c_styp;
   ityp = c1.ityp * c2.ityp;
@@ -110,7 +118,17 @@ instance exportable_ref t {| c:targetlang default_spec t |} : exportable_from (r
   ityp = ref t;
   c_ityp = solve;
   export = (fun x -> x);
-  lemma_export_preserves_prref = (fun _ -> ())
+  lemma_export_preserves_prref = (fun _ -> ());
+}
+
+instance exportable_llist t {| c:exportable_from t |} : exportable_from (linkedList t) = admit ()
+
+instance exportable_refinement t {| c:exportable_from t |} (p:t->Type0) (check:(x:t -> r:bool{r ==> p x})): exportable_from (x:t{p x}) = {
+  c_styp = witnessable_refinement t #c.c_styp p;
+  ityp = c.ityp;
+  c_ityp = c.c_ityp;
+  export = (fun x -> c.export x);
+  lemma_export_preserves_prref = (fun x -> c.lemma_export_preserves_prref x);
 }
 
 instance exportable_arrow 
@@ -119,8 +137,8 @@ instance exportable_arrow
   {| c2:exportable_from t2 |}
   (pre:(t1 -> st_pre))
   (post:(x:t1 -> h0:heap -> st_post' (resexn t2) (pre x h0)))
-  (_:squash (forall x h0 r h1. post x h0 r h1 ==>  post_targetlang_arrow default_spec #(resexn t2) #(witnessable_sum t2 err #c2.c_styp) h0 r h1))
-  (check:(x:t1 -> ST (either unit err) All (fun h0 -> (Mktuple3?._1 default_spec) h0) (fun h0 r h1 -> h0==h1 /\ (Inl? r ==> pre x h0)))) 
+  (_:squash (forall x h0 r h1. post x h0 r h1 ==> post_targetlang_arrow default_spec #(resexn t2) #(witnessable_sum t2 err #c2.c_styp) h0 r h1))
+  (check:(x:t1 -> ST (either unit err) All (pre_targetlang_arrow default_spec #_ #c1.c_styp x) (fun h0 r h1 -> h0==h1 /\ (Inl? r ==> pre x h0)))) 
                              (** ^ the fact that the check has a pre-condition means that the check does not have to enforce it
                                  e.g., the invariant on the heap **)
   : exportable_from (x:t1 -> ST (resexn t2) All (pre x) (post x)) = {
@@ -129,15 +147,13 @@ instance exportable_arrow
   c_ityp = targetlang_arrow default_spec c1.ityp (resexn c2.ityp) #_ #(targetlang_sum default_spec c2.ityp err) ;
   export = (fun (f:(x:t1 -> ST (resexn t2) All (pre x) (post x))) (x:c1.ityp) ->
     match c1.import x with
-    | Inl x -> begin
-      match check x with
+    | Inl x' -> begin
+      c1.lemma_import_preserves_prref x;
+      match check x' with
       | Inl _ -> begin
-        match f x with
-        | Inl r -> begin
-          c2.lemma_export_preserves_prref r; (** the squash + this lemma imply the post-condition **)
-          Inl (c2.export r)
-        end
-        | Inr err -> Inr err
+        let res = f x' in
+        (exportable_resexn t2).lemma_export_preserves_prref res;
+        (exportable_resexn t2).export res
       end
       | Inr err -> Inr err
     end
@@ -219,6 +235,27 @@ instance importable_sum t1 t2 {| c1:importable_to t1 |} {| c2:importable_to t2 |
     | Inr x -> c2.lemma_import_preserves_prref x)
 }
 
+instance safe_importable_ref t {| c:targetlang default_spec t |} : safe_importable_to (ref t) = {
+  c_styp = witnessable_mref t _ #c.wt;
+  ityp = ref t;
+  c_ityp = solve;
+  safe_import = (fun x -> x);
+  lemma_safe_import_preserves_prref = (fun _ -> ())
+}
+
+instance importable_llits t {| c:importable_to t |} : importable_to (linkedList t) = admit ()
+
+instance import_refinement t {| c:importable_to t |} (p:t->Type0) (check:(x:t -> r:bool{r ==> p x})): importable_to (x:t{p x}) = {
+  c_styp = witnessable_refinement t #c.c_styp p;
+  ityp = c.ityp;
+  c_ityp = c.c_ityp;
+  import = (fun x -> 
+    match (c.import x) with
+    | Inl x -> if check x then Inl x else Inr (Contract_failure "check of refinement failed")
+    | Inr err -> Inr err);
+  lemma_import_preserves_prref = (fun x -> c.lemma_import_preserves_prref x);
+}
+
 instance safe_importable_resexn t {| c:importable_to t |} : safe_importable_to (resexn t) = {
   c_styp = witnessable_sum t err #c.c_styp;
   ityp = resexn c.ityp;
@@ -261,8 +298,7 @@ instance safe_importable_arrow
   (pre:(t1 -> st_pre))
   (post:(x:t1 -> h0:heap -> st_post' (resexn t2) (pre x h0)))
   (_:squash (forall (x:t1) h0. pre x h0 ==> pre_targetlang_arrow default_spec #_ #c1.c_styp x h0))
-  (_:squash (forall (x:t1) h0 r h1. pre x h0 /\ post_targetlang_arrow default_spec #_ #(witnessable_sum t2 err #c2.c_styp) h0 r h1 ==> 
-    (forall err. post x h0 (Inr err) h1)))
+  (_:squash (forall (x:t1) h0 e h1. pre x h0 /\ post_targetlang_arrow default_spec #_ #(witnessable_sum t2 err #c2.c_styp) h0 (Inr e) h1 ==> post x h0 (Inr e) h1))
   (capture_check:capture_check t1 (resexn t2) #(witnessable_sum _ err #c2.c_styp) pre post)
   : safe_importable_to (x:t1 -> ST (resexn t2) All (pre x) (post x)) = {
   c_styp = witnessable_arrow t1 (resexn t2) pre post;
@@ -282,9 +318,9 @@ instance safe_importable_arrow
   lemma_safe_import_preserves_prref = (fun _ -> ())
 }
 
-type of_f = x:ref int -> SST (resexn unit) (requires (fun h0 -> satisfy x (Mktuple3?._2 default_spec))) (ensures (fun h0 r h1 -> Inr? r \/ sel h0 x == sel h1 x))
+type f_eqx = x:ref int -> SST (resexn unit) (requires (fun h0 -> satisfy x (Mktuple3?._2 default_spec))) (ensures (fun h0 r h1 -> Inr? r \/ sel h0 x == sel h1 x))
 
-let test : safe_importable_to of_f =
+let f_eqx_is_safe_importable : safe_importable_to f_eqx =
   safe_importable_arrow 
     (ref int) unit
     (fun x -> sst_pre (fun h0 -> satisfy x (Mktuple3?._2 default_spec))) 
@@ -296,7 +332,7 @@ let test : safe_importable_to of_f =
       let x = sst_read' rx in
       let eh0 = get_heap () in
       let check : cb_capture_check (ref int) (resexn unit) _ _ rx eh0 = 
-        (fun res -> if x = sst_read rx then Inl () else Inr (Contract_failure "x is not equal")) in
+        (fun res -> if x = sst_read rx then Inl () else Inr (Contract_failure "x has changed")) in
       (| eh0, check |))
 
 val unsafe_f : mk_targetlang_arrow default_spec (ref int) (resexn unit)
@@ -306,4 +342,26 @@ let unsafe_f x =
   sst_write x 0;
   Inl ()
 
-let safe_f = test.safe_import unsafe_f
+let safe_f = f_eqx_is_safe_importable.safe_import unsafe_f
+
+type f_xeq5 = x:ref int -> SST (resexn int) (requires (fun h0 -> sel h0 x == 5 /\ satisfy x (Mktuple3?._2 default_spec))) (ensures (fun h0 r h1 -> (Inr? r \/ (Inl? r /\ Inl?.v r == 2)) /\ ((Mktuple3?._3 default_spec) h0 h1)))
+  
+let f_xeq5_is_exportable : exportable_from f_xeq5 =
+  exportable_arrow 
+    (ref int) int
+    (fun x -> sst_pre (fun h0 -> sel h0 x == 5 /\ satisfy x (Mktuple3?._2 default_spec))) 
+    (fun x -> sst_post (resexn int) _ (fun h0 r h1 -> (Inr? r \/ (Inl? r /\ Inl?.v r == 2)) /\ ((Mktuple3?._3 default_spec) h0 h1)))
+    ()
+    (fun x ->
+      recall (contains_pred x);
+      if sst_read x = 5 then Inl ()
+      else Inr (Contract_failure "x is not equal to 5"))
+
+val f_with_pre : f_xeq5
+let f_with_pre x = 
+  recall (contains_pred x);
+  let v = sst_read' x in
+  assert (v == 5);
+  Inl (10 / v)
+
+let f_with_dc = f_xeq5_is_exportable.export f_with_pre
